--save_z3_transcript

src/3d/ocaml/Z3.ml
@@ -5,8 +5,21 @@ let tee debug ch s =
   output_string ch s;
   flush ch
 
-let with_z3 (debug: bool) (f: (z3 -> 'a)) : 'a =
+let maybe_output_string (maybe_file: out_channel option) (s: string) =
+  match maybe_file with
+  | None -> ()
+  | Some f -> output_string f s
+
+let maybe_output_line (maybe_file: out_channel option) (s: string) =
+  maybe_output_string maybe_file s;
+  maybe_output_string maybe_file "\n"
+
+let with_z3 (debug: bool) (transcript: string option) (f: (z3 -> 'a)) : 'a =
   let (ch_from_z3, ch_to_z3) as ch_z3 = Unix.open_process (Printf.sprintf "%s -in" (Options.get_z3_executable ())) in
+  let ch_transcript = match transcript with
+    | None -> None
+    | Some f -> Some (open_out f)
+  in
   let valid = ref true in
   let is_from = ref true in
   let from_z3 () : string =
@@ -14,10 +27,13 @@ let with_z3 (debug: bool) (f: (z3 -> 'a)) : 'a =
       if not !is_from
       then begin
         if debug then print_endline ";; From z3";
+        maybe_output_line ch_transcript ";; From z3";
         is_from := true
       end;
       let s = input_line ch_from_z3 in
       if debug then print_endline s;
+      maybe_output_string ch_transcript "; ";
+      maybe_output_line ch_transcript s;
       s
     end
     else ""
@@ -27,8 +43,10 @@ let with_z3 (debug: bool) (f: (z3 -> 'a)) : 'a =
       if !is_from
       then begin
         if debug then print_endline ";; To z3";
+        maybe_output_line ch_transcript ";; To z3";
         is_from := false
       end;
+      maybe_output_line ch_transcript s;
       tee debug ch_to_z3 s
     end
   in
@@ -40,15 +58,19 @@ let with_z3 (debug: bool) (f: (z3 -> 'a)) : 'a =
   let res = f z3 in
   valid := false;
   let _ = Unix.close_process ch_z3 in
+  let _ = match ch_transcript with
+    | None -> ()
+    | Some f -> close_out f
+  in
   res
 
 type z3_thread = int
 
-let with_z3_thread (debug: bool) (f: (z3 -> unit)) : z3_thread =
+let with_z3_thread (debug: bool) (transcript: string option) (f: (z3 -> unit)) : z3_thread =
   let pid = Unix.fork () in
   if pid = 0
   then begin
-    with_z3 debug f;
+    with_z3 debug transcript f;
     exit 0
   end
   else pid
