src/3d/Options.fsti
@@ -75,3 +75,5 @@ val get_z3_witnesses: unit -> ML int
 val get_debug: unit -> ML bool
 
 val get_z3_diff_test: unit -> ML (option (string & string))
+
+val get_save_z3_transcript: unit -> ML (option string)
